

2.3

$$\hat{\sigma}_x = \begin{pmatrix} 0 & 1 \\ 1 & 0 \end{pmatrix} \quad \hat{\sigma}_y = \begin{pmatrix} 0 & -i \\ i & 0 \end{pmatrix}$$

$$\hat{\sigma}_z = \begin{pmatrix} 1 & 0 \\ 0 & -1 \end{pmatrix}$$

a) GIVEN MATRICES \hat{A}, \hat{B} , DEFINE A COMMUTATOR AS:

$$[\hat{A}, \hat{B}] = \hat{A}\hat{B} - \hat{B}\hat{A}$$

$$\bullet \quad [\hat{\sigma}_x, \hat{\sigma}_y] = \begin{pmatrix} 0 & 1 \\ 1 & 0 \end{pmatrix} \begin{pmatrix} 0 & -i \\ i & 0 \end{pmatrix} - \begin{pmatrix} 0 & -i \\ i & 0 \end{pmatrix} \begin{pmatrix} 0 & 1 \\ 1 & 0 \end{pmatrix}$$

$$= \begin{pmatrix} i & 0 \\ 0 & -i \end{pmatrix} - \begin{pmatrix} -i & 0 \\ 0 & i \end{pmatrix}$$

$$= \begin{pmatrix} i+i & 0 \\ 0 & -i-i \end{pmatrix} = 2i \begin{pmatrix} 1 & 0 \\ 0 & -1 \end{pmatrix}$$

$$\bullet \quad [\hat{\sigma}_z, \hat{\sigma}_x] = \begin{pmatrix} 1 & 0 \\ 0 & -1 \end{pmatrix} \begin{pmatrix} 0 & 1 \\ 1 & 0 \end{pmatrix} - \begin{pmatrix} 0 & 1 \\ 1 & 0 \end{pmatrix} \begin{pmatrix} 1 & 0 \\ 0 & -1 \end{pmatrix}$$

$$= \begin{pmatrix} 0 & 1 \\ -1 & 0 \end{pmatrix} - \begin{pmatrix} 0 & -1 \\ 1 & 0 \end{pmatrix}$$

$$= \begin{pmatrix} 0 & 2 \\ -2 & 0 \end{pmatrix} = (-1) \cdot 2 \begin{pmatrix} 0 & -1 \\ 1 & 0 \end{pmatrix}$$

↑
-1 = i²

$$= 2i \begin{pmatrix} 0 & -i \\ i & 0 \end{pmatrix}$$

$$\bullet \quad [\hat{\sigma}_y, \hat{\sigma}_z] = \begin{pmatrix} 0 & -i \\ i & 0 \end{pmatrix} \begin{pmatrix} 1 & 0 \\ 0 & -1 \end{pmatrix} - \begin{pmatrix} 1 & 0 \\ 0 & -1 \end{pmatrix} \begin{pmatrix} 0 & -i \\ i & 0 \end{pmatrix}$$

$$= \begin{pmatrix} 0 & i \\ i & 0 \end{pmatrix} - \begin{pmatrix} 0 & -i \\ -i & 0 \end{pmatrix}$$

$$= \begin{pmatrix} 0 & 2i \\ 2i & 0 \end{pmatrix} = 2i \begin{pmatrix} 0 & 1 \\ 1 & 0 \end{pmatrix} = 2i \hat{\sigma}_x$$

6) CONSIDER $\hat{H} = \mu B \hat{\sigma}_x$, WITH $\mu = e\hbar / (2m\gamma) \sim 0.5 \text{ eV/G}$

HEISENBERG EQ OF MOTION: $\frac{d}{dt} \hat{A}(t) = \left(\frac{i}{\hbar}\right) [\hat{H}, \hat{A}(t)]$ ①

WITH i.c: $\hat{A}(0) = \hat{A}$, DERIVE THE TIME EVOLUTION FOR

$$\hat{\sigma}_z(t)$$

$$\textcircled{1} \rightarrow \frac{d}{dt} \hat{A}(t) = \left(\frac{i}{\hbar}\right) [\mu B \hat{\sigma}_x, \hat{A}(t)]$$

$$\stackrel{\text{UNEQUALITY}}{\neq} \left(\frac{i}{\hbar}\right) \underbrace{\mu B}_{\frac{\omega}{2} = \frac{\mu B}{\hbar}} \left[\frac{\hat{\sigma}_x}{2i}, \hat{A}(t) \right]$$

$$\stackrel{\text{}}{=} \frac{\omega}{4} \left[[\hat{\sigma}_y, \hat{\sigma}_z], \hat{A} \right]$$

$$\bullet 2i \hat{\sigma}_x = [\hat{\sigma}_y, \hat{\sigma}_z]$$

$$= \frac{\omega}{4} \left(- [[\hat{\sigma}_z, \hat{A}] \hat{\sigma}_y] - [[\hat{A}, \hat{\sigma}_z] \hat{\sigma}_y] \right)$$

$$\stackrel{\text{SACREDI IDENTITY}}{\uparrow} \left[\hat{\sigma}_y, \hat{\sigma}_z \right] \hat{A} = - [[\hat{\sigma}_z, \hat{A}] \hat{\sigma}_y] - [[\hat{A}, \hat{\sigma}_z] \hat{\sigma}_y]$$

• EXPAND COMMUTATOR:

$$= \frac{\omega}{4} \left(- \left[\hat{\sigma}_z \hat{A} - \hat{A} \hat{\sigma}_z, \hat{\sigma}_y \right] - \left[\hat{A} \hat{\sigma}_z - \hat{\sigma}_z \hat{A}, \hat{\sigma}_y \right] \right)$$

$$= \frac{\omega}{4} \left(- \left[\hat{\sigma}_z \hat{A}, \hat{\sigma}_y \right] + \left[\hat{A} \hat{\sigma}_z, \hat{\sigma}_y \right] - \left[\hat{A} \hat{\sigma}_z, \hat{\sigma}_y \right] + \left[\hat{\sigma}_z \hat{A}, \hat{\sigma}_y \right] \right)$$

$$\frac{d}{dt} \hat{A}(t) = 0!$$

$$\textcircled{c} \quad \omega = \frac{2\mu B}{\hbar} \quad \text{AND} \quad \nu = \frac{\omega}{2\pi}$$

$$\text{IF } B = 1 \text{ G}$$

$$\Rightarrow \nu = \frac{\omega}{2\pi} = \frac{2\mu B}{2\pi \hbar} = \frac{\mu}{\pi \hbar} \cdot 1 \text{ G}$$

$$= \frac{e\hbar}{2m_e \pi \hbar} \cdot 1 \text{ G} = \frac{1}{2\pi} \frac{e}{m_e} \cdot 1 \text{ G}$$

$$\mu = \frac{e\hbar}{2m_e}$$

$$\Rightarrow \nu = \frac{1 \text{ G}}{2\pi} \cdot \frac{1,602 \cdot 10^{-19} \text{ C}}{9,109 \cdot 10^{-31} \text{ kg}} = 2,799 \cdot 10^{10} \frac{\text{C} \cdot \text{G}}{\text{kg}}$$

$$= 2,799 \cdot 10^6 \frac{\text{C} \cdot \text{T}}{\text{kg}} \rightarrow \frac{\text{A} \cdot \text{s} \cdot \text{kg} \cdot \text{A}^{-1} \cdot \text{s}^{-2}}{\text{kg}}$$

$$= 2,799 \cdot 10^6 \frac{1}{\text{s}} \quad 0,29$$

2.4

$$L = \frac{m_e}{2} |\dot{\vec{x}}|^2 + \frac{e^2}{|\vec{x}|} - \frac{e}{c} \vec{A}(\vec{x}) \cdot \dot{\vec{x}}$$

with $\vec{A} = \frac{1}{2} (\vec{B} \times \vec{x})$

(A) From LAGRANGIAN - D EULER LAGRANGE:

$$\frac{d}{dt} \left(\frac{\partial L}{\partial \dot{x}} \right) = \frac{\partial L}{\partial x}$$

$$\rightarrow \frac{d}{dt} \left(m_e \dot{\vec{x}} - \frac{e}{c} \vec{A}(\vec{x}) \right) = \left(-\frac{e^2}{\vec{x}^2} - \frac{e \dot{\vec{x}}}{c} \frac{\partial \vec{A}(\vec{x})}{\partial \vec{x}} \right)$$

$$\rightarrow m_e \ddot{\vec{x}} - \frac{e}{c} \left(\frac{d}{dt} (\vec{A}(\vec{x})) \right) = -\frac{e^2}{\vec{x}^2} - \frac{e \dot{\vec{x}}}{c} \frac{\partial \vec{A}(\vec{x})}{\partial \vec{x}}$$

CHAIN RULE:

$$\frac{d\vec{A}}{dt} = \underbrace{\frac{\partial \vec{x}}{\partial t}}_{\dot{\vec{x}}} \underbrace{\frac{\partial \vec{A}}{\partial \vec{x}}}_{\partial_i \vec{A}} + \frac{\partial \vec{A}}{\partial t}$$

$$\cdot \partial_j \vec{A}(\vec{x})$$

$$\Rightarrow m_e \ddot{\vec{x}} - \frac{e}{c} \left(\dot{\vec{x}} \partial_i \vec{A} + \frac{\partial \vec{A}}{\partial t} \right) = - \frac{e^2}{\vec{x}^2} - \frac{e}{c} \dot{\vec{x}} \partial_j \vec{A}(x)$$

$$\Rightarrow \underbrace{m_e \ddot{\vec{x}}}_F = \frac{e}{c} \underbrace{\left(\dot{\vec{x}} \partial_i \vec{A} - \partial_j \vec{A} \right)}_{L_D (\dot{\vec{x}} \times \vec{B})} + \frac{e}{c} \frac{\partial \vec{A}}{\partial t} - \frac{e^2}{\vec{x}^2}$$

$$\Rightarrow \vec{F} = \frac{e}{c} (\dot{\vec{x}} \times \vec{B}) + \frac{e}{c} \frac{\partial \vec{A}}{\partial t} - \frac{e^2}{\vec{x}^2}$$

IF WE ASSUME $\frac{e}{|\vec{x}|} = \phi$ SCALAR POTENTIAL, THEN

$$\frac{\partial}{\partial \vec{x}} \phi = -e \frac{1}{\vec{x}^2}$$

$\nabla \phi$

$$\Rightarrow \vec{F} = \frac{e}{c} (\dot{\vec{x}} \times \vec{B}) + \frac{e}{c} \frac{\partial \vec{A}}{\partial t} + e \nabla \phi$$

$c=1$

$$\vec{E} = \left(\frac{\partial \vec{A}}{\partial t} + \nabla \phi \right)$$

$$= e \left(\vec{E} + \dot{\vec{x}} \times \vec{B} \right)$$

b) In TNDUE $\chi = \begin{pmatrix} x \\ y \\ z \end{pmatrix} = r \begin{pmatrix} \sin \theta \cos \phi \\ \sin \theta \sin \phi \\ \cos \theta \end{pmatrix}$

AND $B = (0, 0, B)$

WE WRITE $\vec{A} = \frac{1}{2} (\vec{B} \times \vec{r}) = \frac{1}{2} \begin{pmatrix} 0 \\ 0 \\ B \end{pmatrix} \times \begin{pmatrix} r \sin \theta \cos \phi \\ r \sin \theta \sin \phi \\ r \cos \theta \end{pmatrix}$

$= \frac{1}{2} B r \sin \theta \begin{pmatrix} -\sin \phi \\ \cos \phi \\ 0 \end{pmatrix}$

$\Rightarrow L = \frac{m_e}{2} |\dot{\vec{x}}|^2 + \frac{e^2}{|\vec{x}|} - \frac{e}{c} \vec{A}(\vec{x}) \cdot \dot{\vec{x}}$

\downarrow
SWITCH TO POLAR:

$\vec{x} \equiv \vec{q} = r \hat{r} \rightarrow \dot{\vec{x}} \equiv \dot{\vec{q}} = \dot{r} \hat{r} + r \dot{\theta} \hat{\theta} + r \dot{\phi} \sin \theta \hat{\phi}$

$|\vec{A}| = \sqrt{A_x^2 + A_y^2 + A_z^2}$

$\Rightarrow L = \frac{m_e}{2} (\sqrt{\dot{r}^2 + r^2 \dot{\theta}^2 + r^2 \dot{\phi}^2 \sin^2 \theta})^2 + \frac{e^2}{\sqrt{r^2}} - \frac{e}{c} \begin{pmatrix} A_x \\ A_y \\ A_z \end{pmatrix} \begin{pmatrix} \dot{x} \\ \dot{y} \\ \dot{z} \end{pmatrix}$

$\Rightarrow L = \frac{m_e}{2} (\quad) + \frac{e^2}{r} - \frac{e B r \sin \theta}{2 c} \begin{pmatrix} -\sin \phi \\ \cos \phi \\ 0 \end{pmatrix} \begin{pmatrix} \dot{x} \\ \dot{y} \\ \dot{z} \end{pmatrix} \quad \star$

$= \frac{m_e}{2} (\quad) + \frac{e^2}{r} - \frac{e B r \sin \theta}{2 c} \begin{pmatrix} r \dot{\phi} \sin \theta \end{pmatrix}$

$$\begin{pmatrix} -\sin\phi \\ \cos\phi \\ 0 \end{pmatrix} \begin{pmatrix} \dot{r} \sin\theta \cos\phi + r \dot{\theta} \cos\theta \cos\phi - r \dot{\phi} \sin\theta \sin\phi \\ \dot{r} \sin\theta \sin\phi + r \dot{\theta} \cos\theta \sin\phi + r \dot{\phi} \sin\theta \cos\phi \\ 0 \end{pmatrix}$$

$$= \cancel{\dot{r}^2 \sin^2\theta \sin\phi \cos\phi} - \cancel{r \dot{\theta} \cos\theta \sin\phi \cos\phi} + r \dot{\phi} \sin\theta \sin^2\phi \\ + \cancel{\dot{r}^2 \sin\theta \sin\phi \cos\phi} + \cancel{r \dot{\theta} \cos\theta \sin\phi \cos\phi} + r \dot{\phi} \sin\theta \cos^2\phi$$

\downarrow
 $r \dot{\phi} \sin\theta$

$$\Rightarrow L = \frac{m_e}{2} (\dot{r}^2 + r^2 \dot{\theta}^2 + r^2 \sin^2\theta \dot{\phi}^2) + \frac{e^2}{r} - \frac{eB}{2c} r^2 \dot{\phi} \sin^2\theta$$

REMEMBER THAT $p_i = \frac{\partial L}{\partial \dot{q}_i}$

ASSOCIATED MOMENTUMS:

$$p_r = \frac{\partial L}{\partial \dot{r}} = m_e \dot{r}, \quad p_\phi = m_e r^2 \sin^2\theta \dot{\phi} - \frac{eB}{2c} r^2 \sin^2\theta$$

$$p_\theta = \frac{\partial L}{\partial \dot{\theta}} = m_e r^2 \dot{\theta}, \quad = m_e r^2 \sin^2\theta \left(\dot{\phi} - \frac{eB}{2cm_0} \right)$$

$$\Rightarrow \dot{r} = \frac{p_r}{m_e}, \quad \dot{\theta} = \frac{p_\theta}{m_e r^2}, \quad \dot{\phi} = \frac{p_\phi}{m_e r^2 \sin^2\theta} + \frac{eB}{2cm_0}$$

$$= \frac{2c p_\phi + r^2 \sin^2\theta e B}{2c m_e r^2 \sin^2\theta}$$

REMINDER THAT THE HAMILTONIAN IS:

$$H = p_i \dot{q}_i(p_i, q_i) - L(q_i, \dot{q}_i(p_i, q_i))$$

$$= \frac{p_r^2}{m_e} + \frac{p_\theta^2}{m_e r^2} + \frac{p_\phi^2}{m_e r^2 \sin^2 \theta} + \frac{p_\phi e B}{2 c m_e}$$

$$= \frac{m_e}{2} \left(\frac{p_r^2}{m_e^2} + \cancel{r^2} \frac{p_\theta^2}{m_e^2 \cancel{r^2}} + \frac{p_\phi^2 \cancel{r^2 \sin^2 \theta}}{m_e^2 \cancel{r^2 \sin^2 \theta}} + \frac{e^2 \beta^2 \cancel{r^2 \sin^2 \theta}}{4 c^2 m_e^2} + \frac{2 p_\phi e^2 \beta^2}{2 c m_e^2 \cancel{r^2 \sin^2 \theta}} \right)$$

$$= \frac{e^2}{r} + \frac{e B}{2 c} \cancel{r^2 \sin^2 \theta} \left(\frac{2 c p_\phi + \cancel{r^2 \sin^2 \theta} e B}{2 c m_e \cancel{r^2 \sin^2 \theta}} \right)$$

$$H = \frac{1}{2 m_e} \left(p_r^2 + \frac{1}{r^2} p_\theta^2 + \frac{1}{r^2 \sin^2 \theta} p_\phi^2 \right) + \cancel{\frac{p_\phi e B}{2 c m_e}} - \frac{e^2 B^2 r^2 \sin^2 \theta}{8 c^2 m_e}$$

$$= \cancel{\frac{p_\phi e^2 \beta^2}{2 c m_e}} - \frac{e^2}{r} + \frac{p_\phi e B}{2 c m_e} + \frac{r^2 \sin^2 \theta e^2 \beta^2}{4 c^2 m_e}$$

$$\frac{\cancel{2 r^2 \sin^2 \theta e^2 \beta^2} - \cancel{e^2 \beta^2 r^2 \sin^2 \theta}}{8 c^2 m_e}$$

$$\Rightarrow H = \frac{1}{2 m_e} \left(p_r^2 + \frac{p_\theta^2}{r^2} + \frac{p_\phi^2}{r^2 \sin^2 \theta} \right) - \frac{e^2}{r} + \frac{p_\phi e B}{2 c m_e} + \frac{r^2 \sin^2 \theta e^2 \beta^2}{8 c^2 m_e}$$

P_ϕ is a conserved quantity since the Lagrangian doesn't depend on ϕ :

From E-L

$$\frac{d}{dt} \left[\frac{\partial L}{\partial \dot{\phi}} \right] = \left[\frac{\partial L}{\partial \phi} \right]$$

$$\frac{d}{dt} P_\phi = 0 \quad \text{only if } P_\phi = \text{constant}$$

H is conserved if the system is time invariant: H doesn't

explicitly depend on time.

Since $\frac{\partial H}{\partial t} = 0 \Rightarrow H$ is a conserved quantity

D) $r = \text{BOHR RADIUS}$, $P_\phi = \hbar$, $B \approx 10^5 \text{ G} \sim 10^{15} \text{ G}$

\downarrow \downarrow \downarrow \downarrow
 10^{-11} m 10^{-16} eV.s 10 T 10^{11} T

$m_e = \text{MASS ELECT.}$ $P = \text{MAGNETIC F.}$ $C = \text{LIGHT SPEED}$

\downarrow \downarrow \downarrow
 10^{-31} kg 10^{-19} C 10^8

$v \leq sm \leq \sim \left[\text{ASSUME } v \text{ MAX} \rightarrow 1 \right]$

$$M = \frac{P_r^2}{10^{-31}} + \frac{P_\theta^2}{10^{-53}} + \frac{10^{-31}}{10^{-5321}} + \frac{10^{-38-24}}{10^{-12}} +$$

$$+ \frac{10^{-19} \cdot 10^{-16-4}}{10^{-32} \cdot 10^{87}} + \frac{10^{-38-7} \cdot 10^{-22}}{10^{-31} \cdot 10^{1614}} \rightarrow \frac{10^{-29}}{10^{-12}} \rightarrow 1/10^{43}$$

$$H = \frac{1}{2m_e} \left(P_r^2 + \frac{P_\theta^2}{r^2} + \frac{P_\phi^2}{r^2 s m^2 \theta} \right) - \frac{e^2}{r} + \frac{P_\phi e B}{2 c m_e} + \frac{v^2 s m^2 e^2 B^2}{8 c^2 m_e}$$

\downarrow \downarrow \downarrow \downarrow \downarrow \downarrow
 10^{31} 10^{53} 10^{21} 10^{-17} 10^{-11} 10^{-43}

LAST TERM IS SMALLER BY DIFFERENT POWERS,
AS SUCH WE CAN CONSIDER IT NEGIGIBLE

IN A NEWTON STEP, THE LAST TWO POLYNOMIALS WOULD

BE OF THE MAGNITUDE OF:

$$(1) \frac{1}{10^{11}} \cdot 10^{10} \rightarrow 10^{-1}$$

$$(2) \frac{1}{10^{43}} \cdot 10^{21} \rightarrow 10^{-22}$$

} STILL NEGUGIBLE
COMPARED TO
THE FIRST TERMS

$$e) H = \frac{1}{2m_e} \left(p_r^2 + \frac{p_\theta^2}{r^2} + \frac{p_\phi^2}{r^2 \sin^2 \theta} \right) - \frac{e^2}{r} + \frac{p_\phi e B}{2cm_e}$$

CONSIDER AN ORBIT SUCH THAT $\theta = \pi/2 \rightarrow \sin^2\left(\frac{\pi}{2}\right) = 1$

$$p_\theta = 0$$

SCALAR FIELD $p_\phi = m_\phi \hbar$, $E = H$

$$\bullet \quad E = \frac{1}{2m_e} \left(p_r^2 + \frac{m_\phi^2 \hbar^2}{r^2} \right) - \frac{e^2}{r} + \frac{eB}{2cm_e} m_\phi \hbar$$

$$\Rightarrow p_r = \sqrt{2m_e E - \frac{m_\phi^2 \hbar^2}{r^2} + \frac{2m_e e^2}{r} - \frac{eB m_\phi \hbar}{c}}$$

• EVALUATE SCALAR FIELD CONDITIONS:

$$2 \int_{r_-}^{r_+} p_r dr = m_r \hbar \quad (1)$$

• FROM CONDITION $p_r = 0$ WE FIND:

$$\underline{2m_e E r^2 - m_\phi^2 \hbar^2 + 2m_e e^2 r - eB m_\phi \hbar r^2 = 0}$$

~~$c r^2$~~

$$r^2 \left(2cmE - eB m_\phi \hbar \right) + (2cm e^2)r - cm_\phi^2 \hbar^2 = 0$$

$$r = \frac{-b \pm \sqrt{b^2 - 4ac}}{2a}$$

$$= \frac{-2cm e^2 \pm \sqrt{4c^2 m^2 e^4 + 4cm_\phi^2 \hbar^2 (2cmE - eB m_\phi \hbar)}}{2(2cmE - eB m_\phi \hbar)}$$

Now ① QUANTUMS INTO

$$n_r \hbar = \sqrt{-8meE} \int_{r_-}^{r_+} \frac{1}{r} \sqrt{(r_+ - r)(r - r_-)} dr = \frac{\pi}{2} (\sqrt{r_+} - \sqrt{r_-})^2$$

$$\Rightarrow m_r \hbar = \frac{\pi}{2} \left(\underbrace{r_+ + r_-}_{\downarrow} - \underbrace{\sqrt{r_+} \sqrt{r_-}}_{\downarrow} \right)$$

$$= \frac{-\frac{A+B}{c} + \frac{-A-B}{c}}{c} = \frac{-2A}{c}$$

$$\sqrt{\frac{(-A+B)(-A-B)}{c^2}} \\ \parallel \\ \sqrt{\frac{A^2 - B^2}{c^2}}$$

$$\Rightarrow \frac{2m_r \hbar}{\pi} = \frac{-2A - \sqrt{A^2 - B^2}}{c}$$

$$\frac{2m_r \hbar}{\pi} = \frac{4cm_e e^2 - \sqrt{4c^2 m^2 e^4 - 4c^2 m^2 e^4 + 4cm_\phi^2 \hbar^2 (2cm_e E - eBm_\phi \hbar)}}{2(2cm_e E - eBm_\phi \hbar)}$$

$$\Rightarrow E = - \frac{m_e c^2 \left(\frac{e^2}{\hbar c}\right)^2}{2(m_r + m_\phi)^2} + \frac{eB\hbar m_\phi}{2m_e c}$$